@prefix vf:    <https://w3id.org/valueflows#> .
@prefix schema: <http://schema.org/> .
@prefix rdf:   <http://www.w3.org/1999/02/22-rdf-syntax-ns#> .
@prefix owl:   <http://www.w3.org/2002/07/owl#> .
@prefix skos:  <http://www.w3.org/2004/02/skos/core#> .
@prefix rdfs:  <http://www.w3.org/2000/01/rdf-schema#> .
@prefix foaf:  <http://xmlns.com/foaf/0.1/#> .
@prefix org:   <http://www.w3.org/ns/org#> .
@prefix dcterms: <http://purl.org/dc/terms/> .
@prefix qudt:   <http://qudt.org/schema/qudt/> .
@prefix xsd:   <http://www.w3.org/2001/XMLSchema#> .


<https://w3id.org/valueflows/> a owl:Ontology;
    dcterms:title "Value Flows Ontology";
    dcterms:type <http://purl.org/adms/assettype/Ontology>;
    dcterms:status <http://purl.org/adms/status/UnderDevelopment>.


# ABSTRACT / CLASSIFICATION CLASSES (KNOWLEDGE LAYER)

vf:Action  a           owl:Class ;
        rdfs:label           "vf:Action" ;
        rdfs:subClassOf   rdf:Property ;
        rdfs:comment   "An action verb defining the kind of event, commitment, or intent." .

vf:AgentRelationshipRole  a  owl:Class ;
        rdfs:label           "vf:AgentRelationshipRole" ;
        rdfs:subClassOf   rdf:Property ;
        rdfs:comment   "A relationship role defining the kind of association one agent can have with another." .

vf:ResourceClassification  a    owl:Class ;
        rdfs:label           "vf:ResourceClassification" ;
        rdfs:comment   "A resource category, model, taxonomy item, tag, facet value, or other kind of classification." .

vf:ProcessClassification  a           owl:Class ;
        rdfs:label           "vf:ProcessClassification" ;
        rdfs:comment   "A process category, model, taxonomy item, tag, facet value, or other kind of classification." .

vf:ExchangeClassification  a           owl:Class ;
        rdfs:label           "vf:ExchangeClassification" ;
        rdfs:comment   "An exchange category, model, taxonomy item, tag, facet value, or other kind of classification." .
        
# PLAN CLASSES

#vf:Intent  a       owl:Class ;
#        rdfs:label       "vf:Intent" ;
#        rdfs:comment   "A published want or offer or plan, sometimes with what is expected or desired in return." .

vf:Commitment  a       owl:Class ;
        rdfs:label       "vf:Commitment" ;
        rdfs:comment   "A planned economic event or transfer that has been promised by an agent to another agent." .

vf:Agreement  a       owl:Class ;
        rdfs:label       "vf:Agreement" ;
        rdfs:comment   "Any type of agreement among economic agents, that can be referenced in VF to clarify the economic activity.  This is a placeholder pending investigating other vocabularies." .

vf:ExchangeAgreement  a       owl:Class ;
        rdfs:label       "vf:ExchangeAgreement" ;
        rdfs:subClassOf      vf:Agreement ;
        rdfs:comment   "An agreement to exchange something with another agent(s), containing vf:Commitments towards that end." .

vf:DistributionAgreement  a       owl:Class ;
        rdfs:label        "vf:DistributionAgreement" ;
        rdfs:subClassOf   vf:Agreement ;
        rdfs:comment      "An agreement to distribute some resource in exchange for inputs or outputs created by other agents." .

# OBSERVATION CLASSES


vf:EconomicResource  a           owl:Class ;
        rdfs:label       "vf:EconomicResource" ;
        rdfs:comment   "A resource which is useful to people or the ecosystem." .

vf:Process  a            owl:Class ;
        rdfs:label       "vf:Process" ;
        rdfs:comment   "An activity that changes inputs into outputs.  It could transform or transport vf:EconomicResource(s), as well as simply issuing a resource so that it is available." .

#vf:Transportation  a     owl:Class ;
#        rdfs:label       "vf:Transportation" ;
#        rdfs:subClassOf  vf:Process ;
#        rdfs:comment   "A process that changes the location of a resource(s) without changing the resource(s) itself." .

#vf:Transformation  a     owl:Class ;
#        rdfs:label       "vf:Transformation" ;
#        rdfs:subClassOf  vf:Process ;
#        rdfs:comment   "A process that produces something new from other resources, or improves an existing resource." .

vf:EconomicEvent  a            owl:Class ;
        rdfs:label       "vf:EconomicEvent" ;
        rdfs:comment   "An inflow or outflow of an economic resource in relation to a process and/or exchange. This could reflect a change in the quantity of a vf:EconomicResource. It is also defined by its behavior in relation to the vf:EconomicResource and a vf:Process (consume, use, produce, etc.)" .

foaf:Agent  a                  owl:Class ;
        rdfs:label           "foaf:Agent" ;
        rdfs:comment   "A person or group or organization with economic agency." .

foaf:Person  a                 owl:Class ;
        rdfs:label           "foaf:Person" ;
        rdfs:subClassOf      foaf:Agent ;
        rdfs:comment     "A natural person." .

#foaf:Group  a                  owl:Class ;
#        rdfs:label           "foaf:Group" ;
#        rdfs:subClassOf      foaf:Agent ;
#        rdfs:comment      "Any kind of association of more than one person, which can be loosely or formally organized, but has economic agency as a group beyond any person." .

org:Organization  a         owl:Class ;
        rdfs:label           "org:Organization" ;
        rdfs:subClassOf      foaf:Agent ;
        rdfs:comment      "Usually a more formally defined structure than Group, often legally defined, can be a group or not." .

vf:AgentRelationship  a       owl:Class ;
        rdfs:label       "vf:AgentRelationship" ;
        rdfs:comment    "An ongoing voluntary association between 2 Agents of any kind." .

vf:Fulfillment  a            owl:Class ;
        rdfs:label       "vf:Fulfillment" ;
        rdfs:comment   "The quantity that the vf:EconomicEvent fulfilled towards the vf:Commitment." .

vf:Reciprocity  a        owl:Class ;
        rdfs:label       "vf:Reciprocity" ;
        rdfs:comment     "The quantity that the vf:EconomicEvent implies towards creation of the reciprocal vf:Commitment." .

vf:Appreciation  a            owl:Class ;
        rdfs:label       "vf:Appreciation" ;
        rdfs:comment     "A way to tie an economic event that is given in loose fulfilment for another economic event, without commitments or expectations. Supports the gift economy." .

vf:Location  a           owl:Class ;
        rdfs:label       "vf:Location" .


# not sure about these


#vf:MaterialItem  a       owl:Class ;
#        rdfs:label       "vf:MaterialItem" ;
#        rdfs:subClassOf  vf:Resource .

#vf:Work  a               owl:Class ;
#        rdfs:label       "vf:Work" ;
#        rdfs:subClassOf  vf:Resource .

#vf:Service  a            owl:Class ;
#        rdfs:label       "vf:Service" ;
#        rdfs:subClassOf  vf:Resource .

#vf:Currency  a           owl:Class ;
#        rdfs:label       "vf:Currency" ;
#        rdfs:subClassOf  vf:Resource .


# ####################################################################
# properties

vf:action
        a                   owl:ObjectProperty ;
        rdfs:label         "action" ;
        rdfs:domain         [ owl:unionOf (vf:EconomicEvent vf:Commitment) ] ;
        rdfs:range          vf:Action ;
        rdfs:comment        "Relates a process input or output to a verb, such as consume, produce, work, improve, etc." .

vf:inputOf
        a                   owl:ObjectProperty ;
        rdfs:label         "input of" ;
        rdfs:domain         [ owl:unionOf (vf:EconomicEvent vf:Commitment) ] ;
        rdfs:range          vf:Process .

vf:outputOf
        a                   owl:ObjectProperty ;
        rdfs:label         "output of" ;
        rdfs:domain         [ owl:unionOf (vf:EconomicEvent vf:Commitment) ] ;
        rdfs:range          vf:Process .

vf:inputs
        a                   owl:ObjectProperty ;
        rdfs:label         "inputs" ;
        rdfs:domain         vf:Process ;
        rdfs:range          vf:EconomicEvent .

vf:outputs
        a                   owl:ObjectProperty ;
        rdfs:label         "outputs" ;
        rdfs:domain         vf:Process ;
        rdfs:range          vf:EconomicEvent .

vf:committedInputs
        a                   owl:ObjectProperty ;
        rdfs:label         "committed inputs" ;
        rdfs:domain         vf:Process ;
        rdfs:range          vf:Commitment .

vf:committedOutputs
        a                   owl:ObjectProperty ;
        rdfs:label         "committed outputs" ;
        rdfs:domain         vf:Process ;
        rdfs:range          vf:Commitment .

vf:resourceClassifiedAs
        a                   owl:ObjectProperty ;
        rdfs:label          "resource classified as" ;
        rdfs:domain         [ owl:unionOf (vf:Commitment vf:EconomicResource) ] ;
        rdfs:range          vf:ResourceClassification ;
        rdfs:comment        "A resource's primary classification, as part of describing that resource." .

vf:processClassifiedAs
        a                   owl:ObjectProperty ;
        rdfs:label          "process classified by" ;
        rdfs:domain         vf:Process ;
        rdfs:range          vf:ProcessClassification ;
        rdfs:comment        "The primary classification that describes a process, at any level of granularity." .

vf:exchangeClassifiedAs
        a                   owl:ObjectProperty ;
        rdfs:label          "exchange classified by" ;
        rdfs:domain         vf:ExchangeAgreement ;
        rdfs:range          vf:ExchangeClassification ;
        rdfs:comment        "The primary classification that describes an exchange agreement, at any level of granularity." .

# waiting to do the recipe model

vf:involves
        a                   owl:ObjectProperty ;
        rdfs:label         "involves" ;
        rdfs:domain         vf:Commitment ; 
        rdfs:range          vf:EconomicResource ;
        rdfs:comment        "EconomicResource the Commitment intends or commits to affect. Could be an actual resource or a category or type of resource." .

vf:underlyingResource
        a                   owl:ObjectProperty ;
        rdfs:label         "underlying resource" ;
        rdfs:domain         vf:EconomicResource ;
        rdfs:range          vf:EconomicResource ;
        rdfs:comment        "A more concrete resource upon which a resource is based." .

vf:relationship  a          owl:ObjectProperty ;
        rdfs:label         "relationship" ;
        rdfs:domain         vf:AgentRelationship ;
        rdfs:range          vf:AgentRelationshipClassification ;
        rdfs:comment        "A kind of relationship that exists between 2 agents." .

#vf:commitsTo
#        a                   owl:ObjectProperty ;
#        rdfs:domain         vf:Commitment ;
#        rdfs:range          vf:Intent ;
#        rdfs:comment        "The Intent that an economic agent promises to fulfill." .

vf:affects
        a                   owl:ObjectProperty ;
        rdfs:label         "affects" ;
        rdfs:domain         vf:EconomicEvent ;
        rdfs:range          vf:EconomicResource ;
        rdfs:comment        "The economic resource that is decremented or incremented by the economic event, or just what the economic event is about." .

vf:appreciationOf
        a                   owl:ObjectProperty ;
        rdfs:label         "appreciation of" ;
        rdfs:domain         vf:Appreciation ;
        rdfs:range          vf:EconomicEvent ;
        rdfs:comment        "The economic event being appreciated (gift economy)." .

vf:appreciationWith
        a                   owl:ObjectProperty ;
        rdfs:label         "appreciation with" ;
        rdfs:domain         vf:Appreciation ;
        rdfs:range          vf:EconomicEvent ;
        rdfs:comment        "The economic event implemented in appreciation (gift economy)." .

vf:provider  a       owl:ObjectProperty ;
        rdfs:domain  [ owl:unionOf (vf:EconomicEvent vf:Commitment) ] ;
        rdfs:label   "provider" ;
        rdfs:range   foaf:Agent ;
        rdfs:comment        "The economic agent from whom the intended, committed, or actual economic event is initiated." .

vf:receiver  a       owl:ObjectProperty ;
        rdfs:domain  [ owl:unionOf (vf:EconomicEvent vf:Commitment) ] ;
        rdfs:label   "receiver" ;
        rdfs:range   foaf:Agent ;
        rdfs:comment        "The economic agent whom the intended, committed, or actual economic event is for." .

vf:subject  a        owl:ObjectProperty ;
        rdfs:domain  vf:AgentRelationship ;
        rdfs:label   "subject" ;
        rdfs:range   foaf:Agent ;
        rdfs:comment    "The subject of a relationship between 2 agents." .

vf:object  a         owl:ObjectProperty ;
        rdfs:domain  vf:AgentRelationship ;
        rdfs:label   "object" ;
        rdfs:range   foaf:Agent ;
        rdfs:comment        "The object of a relationship between 2 agents." .

#vf:context  a        owl:ObjectProperty ;
#        rdfs:domain  vf:AgentRelationship ;
#        rdfs:label   "context" ;
#        rdfs:range   foaf:Agent ;
#        rdfs:comment        "The larger context of a relationship between 2 agents, used where the relationship is not relevant outside of that context." .

vf:scope  a          owl:ObjectProperty ;
        rdfs:domain  [ owl:unionOf (vf:EconomicEvent vf:Commitment vf:AgentRelationship) ] ;
        rdfs:label   "scope" ;
        rdfs:range   owl:Thing ;
        rdfs:comment        "The larger boundary or context, used for documenting, accounting, planning, distributing income." .

vf:under  a          owl:ObjectProperty ;
        rdfs:domain  [ owl:unionOf (vf:EconomicEvent vf:Commitment vf:Reciprocity vf:Fulfillment) ] ; 
        rdfs:label   "under" ;
        rdfs:range   vf:Agreement ;
        rdfs:comment        "Reference an agreement between agents which specifies the rules or policies which govern this event." .

#vf:inExchangeFor  a         owl:ObjectProperty ;
#        rdfs:label   "in exchange for" ;
#        rdfs:domain  vf:Commitment ;
#        rdfs:range   vf:EconomicEvent ;
#        rdfs:comment        "References the economic event that generated the commitment, in cases where based on an agreement, an agent commits to some reciprocity if an event occurs." .

vf:createdBy  a        owl:ObjectProperty ;
        rdfs:label   "created by" ;
        rdfs:domain  vf:Reciprocity ;
        rdfs:range   vf:EconomicEvent ;
        rdfs:comment        "References the economic event that fully or partially created the commitment, often based on a prior agreement." .

vf:creates  a        owl:ObjectProperty ;
        rdfs:label   "creates" ;
        rdfs:domain  vf:Reciprocity ;
        rdfs:range   vf:Commitment ;
        rdfs:comment        "References the commitment that was fully or partially created because of the economic event, often based on a prior agreement." .

vf:contains  a       owl:ObjectProperty ;
        rdfs:label   "contains" ;
        rdfs:domain  vf:EconomicResource ;
        rdfs:range   vf:EconomicResource ;
        rdfs:comment        "Used when a stock economic resource contains units also defined as economic resources." .

vf:currentQuantity a owl:ObjectProperty ;
        rdfs:label      "current quantity" ;
        rdfs:domain     vf:EconomicResource ;
        rdfs:range      qudt:QuantityValue ;
        rdfs:comment    "The current amount and unit of the economic resource." .

vf:affectedQuantity a owl:ObjectProperty ;
        rdfs:label      "affected quantity" ;
        rdfs:domain     vf:EconomicEvent ;
        rdfs:range      qudt:QuantityValue ;
        rdfs:comment    "The quantity and unit of the event. This is the quantity that could be used to increment or decrement a resource, depending on the type of resource and type of event." .

vf:fulfilledQuantity a owl:ObjectProperty ;
        rdfs:label      "fulfilled quantity" ;
        rdfs:domain     vf:Fulfillment ;
        rdfs:range      qudt:QuantityValue ;
        rdfs:comment    "The quantity of the fulfillment of an event towards a commitment." .

vf:currentLocation a owl:ObjectProperty ;
        rdfs:label   "current location" ;
        rdfs:domain  vf:EconomicResource ;
        rdfs:range   vf:Location ;
        rdfs:comment        "The current place an economic resource is located.  Could be at any level of granularity, from a town to an address to a warehouse location.  Should be mappable." .

vf:primaryLocation a owl:ObjectProperty ;
        rdfs:label   "primary location" ;
        rdfs:domain  foaf:Agent ;
        rdfs:range   vf:Location ;
        rdfs:comment        "The main place an agent is located, often an address where activities occur and mail can be sent. This is usually a mappable geographic location.  It also could be a website address, as in the case of agents who have no physical location." .

vf:start a owl:ObjectProperty ;
        rdfs:label     "start" ;
        rdfs:domain     vf:EconomicEvent ;
        rdfs:comment   "The starting date and optionally time of the economic event." .

vf:duration a owl:ObjectProperty ;
        rdfs:label     "duration" ;
        rdfs:domain     vf:EconomicEvent ;
        rdfs:comment   "The observed duration of the economic event." .

vf:plannedStart a       owl:ObjectProperty ;
        rdfs:label     "planned start" ;
        rdfs:domain     vf:Process ;
        rdfs:comment   "The planned or estimated date and optionally time of the process." .

vf:plannedDuration a    owl:ObjectProperty ;
        rdfs:label     "planned duration" ;
        rdfs:domain     vf:Process ;
        rdfs:comment   "The planned or estimated duration of the process." .

vf:image a owl:DatatypeProperty ;
        rdfs:label      "image" .

vf:url a owl:DatatypeProperty ;
        rdfs:label      "url" .

vf:name a owl:DatatypeProperty ;
        rdfs:label      "name" ;
        rdfs:comment    "An informal or formal textual identifier for an object. Does not imply uniqueness." .

vf:note a owl:ObjectProperty ;
        rdfs:label      "note" ;
        rdfs:range      skos:note ;
        rdfs:comment    "A textual comment or description." .

vf:trackingIdentifier a owl:AnnotationProperty ;
        rdfs:label "tracking identifier" ;
        rdfs:domain     vf:EconomicResource ;   
        rdfs:comment    "Sometimes called lot number, used for trackable batched resources. Sometimes called serial number, used when each item must have a trackable identifier (like a computer). Could also be used for other unique tracking identifiers needed for resources." .  

vf:fulfilledBy          a owl:ObjectProperty ;
        rdfs:label      "fulfilled by" ;
        rdfs:range      vf:EconomicEvent ;
        rdfs:domain     vf:Fulfillment ;
        rdfs:comment    "The economic event which completely or partially fulfills a commitment." .

vf:fulfills     a owl:ObjectProperty ;
        rdfs:label      "fulfills" ;
        rdfs:range      vf:Commitment ;
        rdfs:domain     vf:Fulfillment ;
        rdfs:comment    "The commitment which is completely or partially fulfilled by an economic event." .

#vf:isFinished  a        owl:DataTypeProperty ;
#        rdfs:domain     [ owl:unionOf (vf:Commitment vf:Process) ] ; 
#        rdfs:label      "is finished" ;
#        rdfs:range      xsd:boolean ;
#        rdfs:comment    "The commitment or process is complete or not." .

# isSubstitutable "Defines if any resources of that type can be freely substituted for any other resource of that type when used, consumed, traded, etc."

# something for models for GTIN, etc. identifiers

# ################################ agent relationship verbs

#vf:memberOf  a              vf:AgentRelationshipRole ;
#        rdfs:label          "member of" .

#vf:partOf  a                vf:AgentRelationshipRole ;
#        rdfs:label          "part of" .

#vf:peerOf  a                vf:AgentRelationshipRole ;
#        rdfs:label          "peer of" .

# ################################ action verbs

vf:increment  a                vf:Action ;
        rdfs:label          "increment" .

vf:decrement  a                vf:Action ;
        rdfs:label          "decrement" .

vf:unload  a                vf:Action ;
        rdfs:label          "unload" ;
        rdfs:subPropertyOf  vf:increment .

vf:load  a                vf:Action ;
        rdfs:label          "load" ;
        rdfs:subPropertyOf  vf:decrement .

vf:consume  a                vf:Action ;
        rdfs:label          "consume" ;
        rdfs:subPropertyOf  vf:decrement .

vf:use  a                vf:Action ;
        rdfs:label          "use" .

vf:work  a                vf:Action ;
        rdfs:label          "work" .

vf:cite  a                vf:Action ;
        rdfs:label          "cite" .

vf:produce  a                vf:Action ;
        rdfs:label          "produce" ;
        rdfs:subPropertyOf  vf:increment .

vf:accept  a                vf:Action ;
        rdfs:label          "accept" .

vf:improve  a                vf:Action ;
        rdfs:label          "improve" .

vf:issue  a                vf:Action ;
        rdfs:label          "issue" ;
        rdfs:subPropertyOf  vf:decrement .

vf:receive  a                vf:Action ;
        rdfs:label          "receive" ;
        rdfs:subPropertyOf  vf:increment .
