@prefix vf:    <https://w3id.org/valueflows#> .
@prefix rdf:   <http://www.w3.org/1999/02/22-rdf-syntax-ns#> .
@prefix owl:   <http://www.w3.org/2002/07/owl#> .
@prefix rdfs:  <http://www.w3.org/2000/01/rdf-schema#> .
@prefix foaf:  <http://xmlns.com/foaf/0.1/#> .
@prefix dcterms: <http://purl.org/dc/terms/> .
@prefix qudt:   <http://qudt.org/schema/qudt/> .
@prefix xsd:   <http://www.w3.org/2001/XMLSchema#> .
@prefix time:  <http://www.w3.org/2006/time#> .
@prefix vs: <http://www.w3.org/2003/06/sw-vocab-status/ns#> .


<https://w3id.org/valueflows/> a owl:Ontology;
    dcterms:title "Value Flows Ontology";
    dcterms:type <http://purl.org/adms/assettype/Ontology>;
    dcterms:status <http://purl.org/adms/status/UnderDevelopment>.


# ABSTRACT / CLASSIFICATION CLASSES (KNOWLEDGE LAYER)

vf:Action  a                 owl:Class ;
        rdfs:label           "vf:Action" ;
        rdfs:subClassOf      rdf:Property ;
        vs:term_status       "unstable" ;
        rdfs:comment         "An action verb defining the kind of event, commitment, or intent." .

vf:AgentRelationshipRole  a  owl:Class ;
        rdfs:label           "vf:AgentRelationshipRole" ;
        rdfs:subClassOf      rdf:Property ;
        vs:term_status       "unstable" ;
        rdfs:comment         "A relationship role defining the kind of association one agent can have with another." .

#vf:Recipe a                owl:Class ;
#        rdfs:label         "vf:Recipe" ;
#        rdfs:comment       "Recipes contain all the info required to create or improve or move a resource." .

vf:ResourceSpecification a  owl:Class ;
        rdfs:label          "vf:ResourceSpecification" ;
        vs:term_status      "unstable" ;
        rdfs:comment        "Specification of a kind of resource. Could define a material item, service, digital item, currency account, etc." .

vf:RecipeProcess a          owl:Class ;
        rdfs:label          "vf:RecipeProcess" ;
        vs:term_status      "unstable" ;
        rdfs:comment        "Specifies the process part of a recipe for use in planning from recipe." .

vf:RecipeFlow a             owl:Class ;
        rdfs:label          "vf:RecipeFlow" ;
        vs:term_status      "unstable" ;
        rdfs:comment        "The linkage between a process recipe, an action that structures a recipe, and a resource specification." .


# PLAN CLASSES

vf:Intent  a                owl:Class ;
        rdfs:label          "vf:Intent" ;
        vs:term_status      "unstable" ;
        rdfs:comment        "A planned economic flow, which can lead to economic events (sometimes through commitments)" .

vf:Commitment  a            owl:Class ;
        rdfs:label          "vf:Commitment" ;
        vs:term_status      "unstable" ;
        rdfs:comment        "A planned economic flow that has been promised by an agent to another agent." .

vf:Satisfaction  a          owl:Class ;
        rdfs:label          "vf:Satisfaction" ;
        vs:term_status      "unstable" ;
        rdfs:comment        "A commitment or economic event that partially or fully satisfies one or more intents." .

vf:Agreement  a             owl:Class ;
        rdfs:label          "vf:Agreement" ;
        vs:term_status      "unstable" ;
        rdfs:comment        "Any type of agreement among economic agents, that can be referenced in VF to clarify the economic activity.  This is a placeholder pending investigating other vocabularies." .

vf:ExchangeAgreement  a     owl:Class ;
        rdfs:label          "vf:ExchangeAgreement" ;
        rdfs:subClassOf     vf:Agreement ;
        vs:term_status      "unstable" ;
        rdfs:comment        "An agreement to exchange something with another agent(s), containing commitments towards that end." .

vf:DistributionAgreement  a  owl:Class ;
        rdfs:label           "vf:DistributionAgreement" ;
        rdfs:subClassOf      vf:Agreement ;
        vs:term_status      "unstable" ;
        rdfs:comment         "An agreement to distribute some resource in exchange for inputs or outputs created by other agents." .

# OBSERVATION CLASSES


vf:EconomicResource  a      owl:Class ;
        rdfs:label          "vf:EconomicResource" ;
        vs:term_status      "unstable" ;
        rdfs:comment        "A resource which is useful to people or the ecosystem." .

vf:Process  a               owl:Class ;
        rdfs:label          "vf:Process" ;
        vs:term_status      "unstable" ;
        rdfs:comment        "An activity that changes inputs into outputs.  It could transform or transport economic resource(s)." .

vf:Transfer  a              owl:Class ;
        rdfs:label          "vf:Transfer" ;
        vs:term_status      "unstable" ;
        rdfs:comment        "An activity that assigns the rights and responsibilities for an economic resource from one agent to another." .

vf:EconomicEvent  a         owl:Class ;
        rdfs:label          "vf:EconomicEvent" ;
        vs:term_status      "unstable" ;
        rdfs:comment        "An observed economic flow, as opposed to a flow planned to happen in the future. This could reflect a change in the quantity of an economic resource. It is also defined by its behavior in relation to the economic resource (see vf:action)" .

vf:AgentRelationship  a     owl:Class ;
        rdfs:label          "vf:AgentRelationship" ;
        vs:term_status      "unstable" ;
        rdfs:comment        "An ongoing voluntary association between 2 agents of any kind." .

vf:Fulfillment  a           owl:Class ;
        rdfs:label          "vf:Fulfillment" ;
        vs:term_status      "unstable" ;
        rdfs:comment        "The quantity that the economic event fulfilled towards the commitment." .

vf:Reciprocity  a           owl:Class ;
        rdfs:label          "vf:Reciprocity" ;
        vs:term_status      "unstable" ;
        rdfs:comment        "The quantity that the economic event implies towards creation of the reciprocal commitment." .

vf:Appreciation  a          owl:Class ;
        rdfs:label          "vf:Appreciation" ;
        vs:term_status      "unstable" ;
        rdfs:comment        "A way to tie an economic event that is given in loose fulfilment for another economic event, without commitments or expectations. Supports the gift economy." .

#vf:Location  a              owl:Class ;
#        vs:term_status      "unstable" ;
#        rdfs:label          "vf:Location" .


# ####################################################################
# properties

vf:action
        a                   owl:ObjectProperty ;
        rdfs:label          "action" ;
        rdfs:domain         [ owl:unionOf (vf:EconomicEvent vf:Commitment vf:Intent vf:RecipeFlow) ] ;
        rdfs:range          vf:Action ;
        vs:term_status      "unstable" ;
        rdfs:comment        "Relates a process input or output to a verb, such as consume, produce, work, improve, etc." .

vf:inputOf
        a                   owl:ObjectProperty ;
        rdfs:label          "input of" ;
        rdfs:domain         [ owl:unionOf (vf:EconomicEvent vf:Commitment vf:Intent) ] ;
        rdfs:range          [ owl:unionOf (vf:Process vf:Transfer) ] ;
        vs:term_status      "unstable" ;
        rdfs:comment        "Relates an input flow to it's node." .

vf:outputOf
        a                   owl:ObjectProperty ;
        rdfs:label          "output of" ;
        rdfs:domain         [ owl:unionOf (vf:EconomicEvent vf:Commitment vf:Intent) ] ;
        rdfs:range          [ owl:unionOf (vf:Process vf:Transfer) ] ;
        vs:term_status      "unstable" ;
        rdfs:comment        "Relates an output flow to it's node." .

vf:recipeInputOf
        a                   owl:ObjectProperty ;
        rdfs:label          "recipe input of" ;
        rdfs:domain         vf:RecipeFlow ;
        rdfs:range          vf:RecipeProcess ;
        vs:term_status      "unstable" ;
        rdfs:comment        "Relates an input flow to it's node in a recipe." .

vf:recipeOutputOf
        a                   owl:ObjectProperty ;
        rdfs:label          "recipe output of" ;
        rdfs:domain         vf:RecipeFlow ;
        rdfs:range          vf:RecipeProcess ;
        vs:term_status      "unstable" ;
        rdfs:comment        "Relates an output flow to it's node in a recipe." .

vf:involves
        a                   owl:ObjectProperty ;
        rdfs:label          "involves" ;
        rdfs:domain         [ owl:unionOf (vf:Commitment vf:Intent) ] ; 
        rdfs:range          vf:EconomicResource ;
        vs:term_status      "unstable" ;
        rdfs:comment        "Economic resource the commitment commits or the intent intends to affect. Could be an actual resource or a classification / specification of resource." .

vf:underlyingResource
        a                   owl:ObjectProperty ;
        rdfs:label          "underlying resource" ;
        rdfs:domain         vf:EconomicResource ;
        rdfs:range          vf:EconomicResource ;
        vs:term_status      "unstable" ;
        rdfs:comment        "A more concrete resource upon which a resource is based." .

vf:relationship  a          owl:ObjectProperty ;
        rdfs:label          "relationship" ;
        rdfs:domain         vf:AgentRelationship ;
        rdfs:range          vf:AgentRelationshipRole ;
        vs:term_status      "unstable" ;
        rdfs:comment        "A kind of relationship that exists between 2 agents." .

vf:affects
        a                   owl:ObjectProperty ;
        rdfs:label          "affects" ;
        rdfs:domain         vf:EconomicEvent ;
        rdfs:range          vf:EconomicResource ;
        vs:term_status      "unstable" ;
        rdfs:comment        "The economic resource that is decremented or incremented by the economic event, or just what the economic event is about." .

vf:appreciationOf
        a                   owl:ObjectProperty ;
        rdfs:label          "appreciation of" ;
        rdfs:domain         vf:Appreciation ;
        rdfs:range          vf:EconomicEvent ;
        vs:term_status      "unstable" ;
        rdfs:comment        "The economic event being appreciated (gift economy)." .

vf:appreciationWith
        a                   owl:ObjectProperty ;
        rdfs:label          "appreciation with" ;
        rdfs:domain         vf:Appreciation ;
        rdfs:range          vf:EconomicEvent ;
        vs:term_status      "unstable" ;
        rdfs:comment        "The economic event implemented in appreciation (gift economy)." .

vf:provider  a              owl:ObjectProperty ;
        rdfs:domain         [ owl:unionOf (vf:EconomicEvent vf:Commitment vf:Intent) ] ;
        rdfs:label          "provider" ;
        rdfs:range          foaf:Agent ;
        vs:term_status      "unstable" ;
        rdfs:comment        "The economic agent from whom the intended, committed, or actual economic event is initiated." .

vf:receiver  a              owl:ObjectProperty ;
        rdfs:domain         [ owl:unionOf (vf:EconomicEvent vf:Commitment vf:Intent) ] ;
        rdfs:label          "receiver" ;
        rdfs:range          foaf:Agent ;
        vs:term_status      "unstable" ;
        rdfs:comment        "The economic agent whom the intended, committed, or actual economic event is for." .

vf:subject  a               owl:ObjectProperty ;
        rdfs:domain         vf:AgentRelationship ;
        rdfs:label          "subject" ;
        rdfs:range          foaf:Agent ;
        vs:term_status      "unstable" ;
        rdfs:comment        "The subject of a relationship between 2 agents." .

vf:object  a                owl:ObjectProperty ;
        rdfs:domain         vf:AgentRelationship ;
        rdfs:label          "object" ;
        rdfs:range          foaf:Agent ;
        vs:term_status      "unstable" ;
        rdfs:comment        "The object of a relationship between 2 agents." .

vf:inScopeOf  a             owl:ObjectProperty ;
        rdfs:domain         owl:Thing ;
        rdfs:label          "in scope of" ;
        rdfs:range          owl:Thing ;
        vs:term_status      "unstable" ;
        rdfs:comment        "Grouping around something to create a boundary or context, used for documenting, accounting, planning." .

vf:under  a                 owl:ObjectProperty ;
        rdfs:domain         [ owl:unionOf (vf:EconomicEvent vf:Commitment vf:Intent vf:Reciprocity vf:Fulfillment ) ] ; 
        rdfs:label          "under" ;
        rdfs:range          vf:Agreement ;
        vs:term_status      "unstable" ;
        rdfs:comment        "Reference to an agreement between agents which specifies the rules or policies or calculations which govern this flow." .

vf:createdBy  a             owl:ObjectProperty ;
        rdfs:label          "created by" ;
        rdfs:domain         vf:Reciprocity ;
        rdfs:range          vf:EconomicEvent ;
        vs:term_status      "unstable" ;
        rdfs:comment        "References the economic event that fully or partially created the commitment, often based on a prior agreement." .

vf:creates  a               owl:ObjectProperty ;
        rdfs:label          "creates" ;
        rdfs:domain         vf:Reciprocity ;
        rdfs:range          vf:Commitment ;
        vs:term_status      "unstable" ;
        rdfs:comment        "References the commitment that was fully or partially created because of the economic event, often based on a prior agreement." .

vf:contains  a              owl:ObjectProperty ;
        rdfs:label          "contains" ;
        rdfs:domain         vf:EconomicResource ;
        rdfs:range          vf:EconomicResource ;
        vs:term_status      "unstable" ;
        rdfs:comment        "Used when a stock economic resource contains units also defined as economic resources." .

vf:currentQuantity a        owl:ObjectProperty ;
        rdfs:label          "current quantity" ;
        rdfs:domain         vf:EconomicResource ;
        rdfs:range          qudt:QuantityValue ;
        vs:term_status      "unstable" ;
        rdfs:comment        "The current amount and unit of the economic resource. This can be stored or derived from economic events affecting the resource" .

vf:affectedQuantity a       owl:ObjectProperty ;
        rdfs:label          "affected quantity" ;
        rdfs:domain         vf:EconomicEvent ;
        rdfs:range          qudt:QuantityValue ;
        vs:term_status      "unstable" ;
        rdfs:comment        "The quantity and unit of the event. This is the quantity that could be used to increment or decrement a resource, depending on the type of resource and type of event." .

vf:fulfilledQuantity a      owl:ObjectProperty ;
        rdfs:label          "fulfilled quantity" ;
        rdfs:domain         vf:Fulfillment ;
        rdfs:range          qudt:QuantityValue ;
        vs:term_status      "unstable" ;
        rdfs:comment        "The quantity of the fulfillment of an event towards a commitment or an intent." .

vf:satisfiedQuantity a      owl:ObjectProperty ;
        rdfs:label          "satisfied quantity" ;
        rdfs:domain         vf:Satisfaction ;
        rdfs:range          qudt:QuantityValue ;
        vs:term_status      "unstable" ;
        rdfs:comment        "The quantity of the satisfaction of an commitment towards an intent." .

vf:reciprocalQuantity a     owl:ObjectProperty ;
        rdfs:label          "reciprocal quantity" ;
        rdfs:domain         vf:Reciprocity ;
        rdfs:range          qudt:QuantityValue ;
        vs:term_status      "unstable" ;
        rdfs:comment        "The quantity of the reciprocity when an event creates a commitment." .

vf:definedQuantity a        owl:ObjectProperty ;
        rdfs:label          "defined quantity" ;
        rdfs:domain         vf:RecipeFlow ;
        rdfs:range          qudt:QuantityValue ;
        vs:term_status      "unstable" ;
        rdfs:comment        "The amount and unit defined for this recipe flow." .

vf:currentLocation a        owl:ObjectProperty ;
        rdfs:label          "current location" ;
        rdfs:domain         vf:EconomicResource ;
        #rdfs:range          vf:Location ;
        vs:term_status      "unstable" ;
        rdfs:comment        "The current place an economic resource is located.  Could be at any level of granularity, from a town to an address to a warehouse location.  Usually mappable." .

vf:primaryLocation a        owl:ObjectProperty ;
        rdfs:label          "primary location" ;
        rdfs:domain         foaf:Agent ;
        #rdfs:range          vf:Location ;
        vs:term_status      "unstable" ;
        rdfs:comment        "The main place an agent is located, often an address where activities occur and mail can be sent. This is usually a mappable geographic location.  It also could be a website address, as in the case of agents who have no physical location." .

vf:observedTime a           owl:ObjectProperty ;
        rdfs:label          "observed time" ;
        rdfs:domain         vf:EconomicEvent ;
        rdfs:range          time:TemporalEntity ;
        vs:term_status      "unstable" ;
        rdfs:comment        "The actual temporal instant or interval." .

vf:committedTime a          owl:ObjectProperty ;
        rdfs:label          "committed time" ;
        rdfs:domain         vf:Commitment ;
        rdfs:range          time:TemporalEntity ;
        vs:term_status      "unstable" ;
        rdfs:comment        "The promised temporal instant or interval." .

vf:intendedTime a           owl:ObjectProperty ;
        rdfs:label          "intended time" ;
        rdfs:domain         vf:Intent ;
        rdfs:range          time:TemporalEntity ;
        vs:term_status      "unstable" ;
        rdfs:comment        "The intended temporal instant or interval." .

vf:plannedTime a            owl:ObjectProperty ;
        rdfs:label          "planned time" ;
        rdfs:domain         vf:Process ;
        rdfs:range          time:TemporalEntity ;
        vs:term_status      "unstable" ;
        rdfs:comment        "The planned or estimated calendar time the process will take (whether being actually worked or not)." .

vf:image a                  owl:DatatypeProperty ;
        vs:term_status      "unstable" ;
        rdfs:label          "image" .

vf:url a                    owl:DatatypeProperty ;
        vs:term_status      "unstable" ;
        rdfs:label          "url" .

vf:name a                   owl:DatatypeProperty ;
        rdfs:label          "name" ;
        vs:term_status      "unstable" ;
        rdfs:comment        "An informal or formal textual identifier for an object. Does not imply uniqueness." .

vf:trackingIdentifier a     owl:AnnotationProperty ;
        rdfs:label          "tracking identifier" ;
        rdfs:domain         vf:EconomicResource ;   
        vs:term_status      "unstable" ;
        rdfs:comment        "Sometimes called lot number, used for trackable batched resources. Sometimes called serial number, used when each item must have a trackable identifier (like a computer). Could also be used for other unique tracking identifiers needed for resources." .  

vf:fulfilledBy              a owl:ObjectProperty ;
        rdfs:label          "fulfilled by" ;
        rdfs:range          vf:EconomicEvent ;
        rdfs:domain         vf:Fulfillment ;
        vs:term_status      "unstable" ;
        rdfs:comment        "The economic event which completely or partially fulfills a commitment." .

vf:fulfills  a              owl:ObjectProperty ;
        rdfs:label          "fulfills" ;
        rdfs:range          vf:Commitment ;
        rdfs:domain         vf:Fulfillment ;
        vs:term_status      "unstable" ;
        rdfs:comment        "The commitment which is completely or partially fulfilled by an economic event." .

vf:satisfies
        a                   owl:ObjectProperty ;
        rdfs:label         "satisfies" ;
        rdfs:domain         vf:Satisfaction ;
        rdfs:range          vf:Intent ;
        vs:term_status      "unstable" ;
        rdfs:comment        "An intent satisfied fully or partially by an economic event or commitment." .

vf:satisfiedBy
        a                   owl:ObjectProperty ;
        rdfs:label         "satisfied by" ;
        rdfs:domain         vf:Satisfaction ;
        rdfs:range          [ owl:unionOf (vf:Commitment vf:EconomicEvent ) ] ;
        vs:term_status      "unstable" ;
        rdfs:comment        "A commitment or economic event fully or partially satisfying an intent" .

vf:finished  a              owl:DatatypeProperty ;
        rdfs:domain         [ owl:unionOf (vf:Commitment vf:Process vf:Intent) ] ; 
        rdfs:label          "finished" ;
        rdfs:range          xsd:boolean ;
        vs:term_status      "unstable" ;
        rdfs:comment        "The commitment or intent or process is complete or not." .

vf:substitutable a        owl:DatatypeProperty ;
        rdfs:label          "substitutable" ;
        rdfs:domain         vf:ResourceSpecification ;
        rdfs:range          xsd:boolean ;
        vs:term_status      "unstable" ;
        rdfs:comment        "Defines if any resource of that type can be freely substituted for any other resource of that type when used, consumed, traded, etc." .

vf:unit a                   owl:ObjectProperty ;
        rdfs:label          "unit" ;
        rdfs:domain         vf:ResourceSpecification ;
        rdfs:range          qudt:unit ;
        vs:term_status      "unstable" ;
        rdfs:comment        "The unit expected for this resource specification as a default." .

# TODO: need to define this, something like currency, inventory, skill, service; may be other aspects too.
#vf:resourceCategory a    owl:ObjectProperty ;
#        rdfs:label      "category" ;
#        rdfs:domain     vf:ResourceSpecification ;
#        vs:term_status      "unstable" ;
#        rdfs:comment    "Defines the category of behavior expected for the type of resource." .

#vf:variantOf a          owl:ObjectProperty ;
#        rdfs:label      "variant of" ;
#        rdfs:domain     vf:Recipe ;
#        rdfs:range      vf:Recipe ;
#        vs:term_status      "unstable" ;
#        rdfs:comment    "This recipe is a variation of another recipe." .

#vf:successorOf a        owl:ObjectProperty ;
#        rdfs:label      "successor of" ;
#        rdfs:domain     vf:Recipe ;
#        rdfs:range      vf:Recipe ;
#        vs:term_status      "unstable" ;
#        rdfs:comment    "This recipe is an updated version of another recipe." .

vf:duration a               owl:ObjectProperty ;
        rdfs:label          "duration" ;
        rdfs:domain         vf:RecipeProcess ;
        rdfs:range          time:TemporalDuration ;
        vs:term_status      "unstable" ;
        rdfs:comment        "The calendar duration defined for this type of process." .

vf:durationMultiplier 
        a                   owl:DatatypeProperty ;
        rdfs:label          "duration multiplier" ;
        rdfs:domain         vf:RecipeProcess ;
        rdfs:range          xsd:float ;
        vs:term_status      "unstable" ;
        rdfs:comment        "The multiplier for duration based on capacities for the recipe." .

vf:basedOn
        a                   owl:ObjectProperty ;
        rdfs:label          "based on" ;
        rdfs:domain         vf:Process ;
        rdfs:range          vf:RecipeProcess ;
        vs:term_status      "unstable" ;
        rdfs:comment        "The recipe definition or specification for a process." .

vf:classifiedAs
        a                   owl:ObjectProperty ;
        rdfs:label          "classified as" ;
        rdfs:domain         owl:Thing ;
        rdfs:range          owl:Thing ;
        vs:term_status      "unstable" ;
        rdfs:comment        "References a concept in a common taxonomy or other classification scheme for purposes of categorization." .

vf:resourceClassifiedAs
        a                   owl:ObjectProperty ;
        rdfs:label          "resource classified as" ;
        rdfs:domain         [ owl:unionOf (vf:ResourceSpecification vf:Intent vf:Commitment vf:EconomicEvent vf:RecipeFlow) ] ;
        rdfs:range          owl:Thing ;
        vs:term_status      "unstable" ;
        rdfs:comment        "References a concept in a common taxonomy or other classification scheme for purposes of categorization." .

vf:processClassifiedAs
        a                   owl:ObjectProperty ;
        rdfs:label          "process classified as" ;
        rdfs:domain         vf:RecipeProcess ;
        rdfs:range          owl:Thing ;
        vs:term_status      "unstable" ;
        rdfs:comment        "References a concept in a common taxonomy or other classification scheme for purposes of categorization." .

vf:resourceConformsTo
        a                   owl:ObjectProperty ;
        rdfs:label          "resource conforms to" ;
        rdfs:domain         [ owl:unionOf (vf:Commitment vf:EconomicResource vf:Intent vf:RecipeFlow vf:EconomicEvent ) ] ;
        rdfs:range          vf:ResourceSpecification ;
        vs:term_status      "unstable" ;
        rdfs:comment        "The primary resource knowledge specification or definition of an existing or potential resource." .



# ################################ agent relationship verbs

#vf:memberOf  a              vf:AgentRelationshipRole ;
#        vs:term_status      "unstable" ;
#        rdfs:label          "member of" .

#vf:partOf  a                vf:AgentRelationshipRole ;
#        vs:term_status      "unstable" ;
#        rdfs:label          "part of" .

#vf:peerOf  a                vf:AgentRelationshipRole ;
#        vs:term_status      "unstable" ;
#        rdfs:label          "peer of" .

# ################################ action verbs

vf:increment  a             vf:Action ;
        vs:term_status      "unstable" ;
        rdfs:label          "increment" .

vf:decrement  a             vf:Action ;
        vs:term_status      "unstable" ;
        rdfs:label          "decrement" .

vf:unload  a                vf:Action ;
        rdfs:label          "unload" ;
        vs:term_status      "unstable" ;
        rdfs:subPropertyOf  vf:increment .

vf:load  a                  vf:Action ;
        rdfs:label          "load" ;
        vs:term_status      "unstable" ;
        rdfs:subPropertyOf  vf:decrement .

vf:consume  a               vf:Action ;
        rdfs:label          "consume" ;
        vs:term_status      "unstable" ;
        rdfs:subPropertyOf  vf:decrement .

vf:use  a                   vf:Action ;
        vs:term_status      "unstable" ;
        rdfs:label          "use" .

vf:work  a                  vf:Action ;
        vs:term_status      "unstable" ;
        rdfs:label          "work" .

vf:cite  a                  vf:Action ;
        vs:term_status      "unstable" ;
        rdfs:label          "cite" .

vf:produce  a               vf:Action ;
        rdfs:label          "produce" ;
        vs:term_status      "unstable" ;
        rdfs:subPropertyOf  vf:increment .

vf:accept  a                vf:Action ;
        vs:term_status      "unstable" ;
        rdfs:label          "accept" .

vf:improve  a                vf:Action ;
        vs:term_status      "unstable" ;
        rdfs:label          "improve" .

vf:give  a                  vf:Action ;
        rdfs:label          "give" ;
        vs:term_status      "unstable" ;
        rdfs:subPropertyOf  vf:decrement .

vf:receive  a                vf:Action ;
        rdfs:label          "receive" ;
        vs:term_status      "unstable" ;
        rdfs:subPropertyOf  vf:increment .

vf:raise  a                 vf:Action ;
        rdfs:label          "raise" ;
        rdfs:subPropertyOf  vf:increment .

vf:lower  a                 vf:Action ;
        rdfs:label          "lower" ;
        rdfs:subPropertyOf  vf:decrement .
