@base              <https://w3id.org/valueflows/ont/vf> .
@prefix vf:        <#> .
@prefix as:        <https://www.w3.org/ns/activitystreams#> .
@prefix cc:        <http://creativecommons.org/ns#> .
@prefix dcterms:   <http://purl.org/dc/terms/> .
@prefix dtype:     <http://www.linkedmodel.org/schema/dtype#> .
@prefix foaf:      <http://xmlns.com/foaf/0.1/> .
@prefix geo:       <http://www.w3.org/2003/01/geo/wgs84_pos#> .
@prefix geosparql: <http://www.opengis.net/ont/geosparql#> .
@prefix om:        <http://www.ontology-of-units-of-measure.org/resource/om-2/> .
@prefix org:       <http://www.w3.org/ns/org#> .
@prefix owl:       <http://www.w3.org/2002/07/owl#> .
@prefix rdf:       <http://www.w3.org/1999/02/22-rdf-syntax-ns#> .
@prefix rdfs:      <http://www.w3.org/2000/01/rdf-schema#> .
@prefix skos:      <http://www.w3.org/2004/02/skos/core#> .
@prefix spdxt:     <http://spdx.org/rdf/terms#> .
@prefix spdxl:     <https://spdx.org/licenses/> .
@prefix time:      <http://www.w3.org/2006/time#> .
@prefix vann:      <http://purl.org/vocab/vann/> .
@prefix vs:        <http://www.w3.org/2003/06/sw-vocab-status/ns#> .
@prefix xsd:       <http://www.w3.org/2001/XMLSchema#> .

<> a owl:Ontology ;
    dcterms:title "Valueflows Ontology" ;
    dcterms:description "A vocabulary for the distributed economic networks of the next economy, to coordinate the creation, distribution, and exchange of economic resources" ;
    dcterms:type <http://purl.org/adms/assettype/Ontology> ;
    vann:preferredNamespacePrefix "vf" ;
    vann:preferredNamespaceUri "https://w3id.org/valueflows/ont/vf#" ;
    owl:versionInfo "0.17" ;
    owl:versionIRI <https://w3id.org/valueflows/ont/0.17/vf> ;
    dcterms:status <http://purl.org/adms/status/UnderDevelopment> ;
    dcterms:license "https://creativecommons.org/licenses/by-sa/4.0/" ;
    cc:license "https://creativecommons.org/licenses/by-sa/4.0/" ;
    spdxt:licenseDeclared spdxl:CC-BY-SA-4.0 ;
    dcterms:source "https://codeberg.org/valueflows/pages/src/branch/main/assets/all_vf.TTL" ;
    .

vf:Action  a                owl:Class ;
        rdfs:label          "Action"@en ;
        vf:layer            vf:knowledge ;
        vs:term_status      "stable" ;
        rdfs:comment        "An action verb defining the kind of flow and its behavior."@en ;
        .

vf:Agent  a                 owl:Class ;
        rdfs:seeAlso        foaf:Agent ;
        rdfs:label          "Agent"@en ;
        vf:layer            vf:observation ;
        vs:term_status      "stable" ;
        rdfs:comment        "An identifiable entity that can commit to and/or perform economic and/or ecological activity under its own power or authority."@en ;
        .

vf:Agreement  a             owl:Class ;
        rdfs:label          "Agreement"@en ;
        vf:layer            vf:planning ;
        vs:term_status      "stable" ;
        rdfs:comment        "A set of reciprocal commitments among economic agents, or a set of reciprocal economic events."@en ;
        .

vf:AgreementBundle  a       owl:Class ;
        rdfs:label          "Agreement Bundle"@en ;
        vf:layer            vf:planning ;
        vs:term_status      "unstable" ;
        rdfs:comment        "A grouping of agreements to bundle detailed line item reciprocity."@en ;
        .

vf:BatchLotRecord  a        owl:Class ;
        rdfs:label          "Batch Lot Record"@en ;
        vf:layer            vf:observation ;
        vs:term_status      "testing" ;
        rdfs:comment        "A document which contains all the needed detail related to the production process of a particular batch or lot, a resource processed in the same process(es) so that it is expected to be homogeneous."@en ;
        .

vf:Commitment  a            owl:Class ;
        rdfs:label          "Commitment"@en ;
        vf:layer            vf:planning ;
        vs:term_status      "stable" ;
        rdfs:comment        "A planned economic flow that has been scheduled or promised by one agent to another agent."@en ;
        .

vf:EcologicalAgent  a       owl:Class ;
        rdfs:label          "Ecological Agent"@en ;
        vf:layer            vf:observation ;
        rdfs:subClassOf     vf:Agent ;
        vs:term_status      "testing" ;
        rdfs:comment        "A non-human being; or a functional group of non-human beings; or an ecosystem of living beings that includes non-humans; but it has agency and receives and/or provides economic/ecological resources."@en ;
        .

vf:EconomicEvent  a         owl:Class ;
        rdfs:label          "Economic Event"@en ;
        vf:layer            vf:observation ;
        vs:term_status      "stable" ;
        rdfs:comment        "An observed economic flow, which could reflect creation or a change in the quantity, location, accountability and/or responsibility, of an economic resource, whether material or not."@en ;
        .

vf:EconomicResource  a      owl:Class ;
        rdfs:label          "Economic Resource"@en ;
        vf:layer            vf:observation ;
        vs:term_status      "stable" ;
        rdfs:comment        "Economic or environmental things (material or digital), media of exchange, which agents agree should be accounted for and which can be inventoried."@en ;
        .

vf:Intent  a                owl:Class ;
        rdfs:label          "Intent"@en ;
        vf:layer            vf:planning ;
        vs:term_status      "stable" ;
        rdfs:comment        "A desired or proposed or planned or estimated economic flow, usually with only one agent associated, which could become a commitment and/or economic event."@en ;
        .

vf:Measure a                owl:Class ;
        rdfs:subClassOf     om:Measure ;
        rdfs:label          "Measure"@en ;
        vf:layer            vf:utility ;
        vs:term_status      "stable" ;
        rdfs:comment        "A quantity expressed as a numeric value with a unit of measure."@en ;
        .

vf:Organization  a          owl:Class ;
        rdfs:seeAlso        org:Organization ;
        rdfs:label          "Organization"@en ;
        vf:layer            vf:observation ;
        rdfs:subClassOf     vf:Agent ;
        vs:term_status      "stable" ;
        rdfs:comment        "A functional structure, formal or informal, which can include people and/or other organizations, and has its own agency.  Something called a group is an Organization in Valueflows if it has agency as the group."@en ;
        .

vf:Person  a                owl:Class ;
        rdfs:seeAlso        foaf:Person ;
        rdfs:label          "Person"@en ;
        vf:layer            vf:observation ;
        rdfs:subClassOf     vf:Agent ;
        vs:term_status      "stable" ;
        rdfs:comment        "A human being. All persons are considered agents."@en ;
        .

vf:Plan  a                  owl:Class ;
        rdfs:label          "Plan"@en ;
        vf:layer            vf:planning ;
        vs:term_status      "stable" ;
        rdfs:comment        "A logical collection of processes, with optional connected agreements, that constitute a body of scheduled work with defined deliverable(s)."@en ;
        .

vf:Process  a               owl:Class ;
        rdfs:label          "Process"@en ;
        vf:layer            vf:observation ;
        vs:term_status      "stable" ;
        rdfs:comment        "An activity that changes inputs into outputs, by transforming or transporting economic resource(s)."@en ;
        .

vf:ProcessSpecification a   owl:Class ;
        rdfs:label          "Process Specification"@en ;
        vf:layer            vf:knowledge ;
        vs:term_status      "stable" ;
        rdfs:comment        "Specifies the kind of process, and also the stage of the process."@en ;
        .

vf:Proposal  a              owl:Class ;
        rdfs:label          "Proposal"@en ;
        vf:layer            vf:planning ;
        vs:term_status      "stable" ;
        rdfs:comment        "Published requests or offers, sometimes with what is expected in return."@en ;
        .

vf:ProposalList  a          owl:Class ;
        rdfs:label          "Proposal List"@en ;
        vf:layer            vf:planning ;
        vs:term_status      "unstable" ;
        rdfs:comment        "A grouping of proposals, for publishing as a list."@en ;
        .

vf:Recipe a                 owl:Class ;
        rdfs:label          "Recipe"@en ;
        vf:layer            vf:knowledge ;
        vs:term_status      "testing" ;
        rdfs:comment        "Optional instance of a recipe which directly specifies the recipe processes included."@en ;
        .

vf:RecipeExchange a         owl:Class ;
        rdfs:label          "Recipe Exchange"@en ;
        vf:layer            vf:knowledge ;
        vs:term_status      "stable" ;
        rdfs:comment        "Specifies an exchange type agreement as part of a recipe."@en ;
        .

vf:RecipeFlow a             owl:Class ;
        rdfs:label          "Recipe Flow"@en ;
        vf:layer            vf:knowledge ;
        vs:term_status      "stable" ;
        rdfs:comment        "The specification of a resource inflow to, or outflow from, a recipe process; and/or a clause, or reciprocal clause, of a recipe exchange."@en ;
        .

vf:RecipeProcess a          owl:Class ;
        rdfs:label          "Recipe Process"@en ;
        vf:layer            vf:knowledge ;
        vs:term_status      "stable" ;
        rdfs:comment        "Specifies a process in a recipe for use in planning from recipe."@en ;
        .

vf:ResourceSpecification a  owl:Class ;
        rdfs:label          "Resource Specification"@en ;
        vf:layer            vf:knowledge ;
        vs:term_status      "stable" ;
        rdfs:comment        "Specifies the kind of economic or environmental resource, even if the resource is not instantiated as an EconomicResource. Could define a material or digital thing, service, medium of exchange or currency, skill or type of work."@en ;
        .

vf:SpatialThing a           owl:Class ;
        rdfs:subClassOf     geo:SpatialThing ;
        rdfs:label          "Spatial Thing"@en ;
        vf:layer            vf:utility ;
        vs:term_status      "stable" ;
        rdfs:comment        "Data that locates something relative to the Earth, usually a somewhat fixed location."@en ;
        .

vf:Unit a                   owl:Class ;
        rdfs:subClassOf     om:Unit ;
        rdfs:label          "Unit"@en ;
        vf:layer            vf:utility ;
        vs:term_status      "stable" ;
        rdfs:comment        "A standard unit of measure, defined and adopted by convention or by law."@en ;
        .

vf:accountingQuantity a     owl:ObjectProperty ;
        rdfs:label          "accounting quantity"@en ;
        rdfs:domain         vf:EconomicResource ;
        rdfs:range          vf:Measure ;
        owl:maxCardinality  1 ;
        vs:term_status      "stable" ;
        rdfs:comment        "The current amount and unit of the economic resource for which the agent has primary rights and responsibilities, sometimes thought of as ownership. This can be either stored or derived from economic events affecting the resource."@en ;
        .

vf:action
        a                   owl:ObjectProperty ;
        rdfs:label          "action"@en ;
        rdfs:domain         [ owl:unionOf (vf:EconomicEvent vf:Commitment vf:Intent vf:RecipeFlow vf:Claim) ] ;
        rdfs:range          vf:Action ;
        owl:cardinality     1 ;
        vs:term_status      "stable" ;
        rdfs:comment        "Defines the kind of flow, such as consume, produce, work, transfer, etc."@en ;
        .

vf:alt a                    owl:DatatypeProperty ;
        rdfs:subPropertyOf  geo:alt ;
        rdfs:range          dtype:numericUnion ;
        rdfs:domain         vf:SpatialThing ;
        owl:maxCardinality  1 ;
        vs:term_status      "testing" ;
        rdfs:comment        "The WGS84 altitude of a spatial thing (decimal meters above the local reference ellipsoid)" ;
        .

vf:availableQuantity a      owl:ObjectProperty ;
        rdfs:label          "available quantity"@en ;
        rdfs:domain         vf:Intent ;
        rdfs:range          vf:Measure ;
        owl:maxCardinality  1 ;
        vs:term_status      "stable" ;
        rdfs:comment        "The amount and unit of the offered resource currently available."@en ;
        .

vf:batchLotCode a           owl:DatatypeProperty ;
        rdfs:label          "batch or lot code"@en ;
        rdfs:domain         vf:BatchLotRecord ;
        rdfs:range          xsd:string ;
        owl:maxCardinality  1 ;
        vs:term_status      "testing" ;
        rdfs:comment        "The code or identifier for this batch or lot, used to physically label individuals in the batch or lot."@en ;
        .

vf:bundledIn a              owl:ObjectProperty ;
        rdfs:label          "bundled in"@en ;
        rdfs:domain         vf:Agreement ;
        rdfs:range          vf:AgreementBundle ;
        owl:maxCardinality  1 ;
        vs:term_status      "testing" ;
        rdfs:comment        "This agreement is bundled with other agreements, for example in an order."@en ;
        .

vf:bundles a                owl:ObjectProperty ;
        owl:inverseOf       vf:bundledIn ;
        rdfs:label          "bundles"@en ;
        rdfs:domain         vf:AgreementBundle ;
        rdfs:range          vf:Agreement ;
        vs:term_status      "testing" ;
        rdfs:comment        "All the agreements included in this agreement bundle."@en ;
        .

vf:basedOn
        a                   owl:ObjectProperty ;
        rdfs:label          "based on"@en ;
        rdfs:domain         vf:Process ;
        rdfs:range          vf:ProcessSpecification ;
        owl:maxCardinality  1 ;
        vs:term_status      "stable" ;
        rdfs:comment        "The definition or standard specification for a process."@en ;
        .

vf:classifiedAs
        a                   owl:ObjectProperty ;
        rdfs:label          "classified as"@en ;
        rdfs:domain         [ owl:unionOf (vf:Process vf:EconomicResource vf:Organization vf:EcologicalAgent vf:Unit) ] ;
        rdfs:range          xsd:string ;
        vs:term_status      "unstable" ;
        rdfs:comment        "References one or more uri's for a concept in a common taxonomy or other classification scheme for purposes of categorization or grouping; or it can be one or more string classifications such as tags."@en ;
        .

vf:clauseOf a               owl:ObjectProperty ;
        rdfs:label          "clause of"@en ;
        rdfs:domain         vf:Commitment ;
        rdfs:range          vf:Agreement ;
        owl:maxCardinality  1 ;
        vs:term_status      "stable" ;
        rdfs:comment        "This commitment is a primary part of the agreement."@en ;
        .

vf:conformsTo
        a                   owl:ObjectProperty ;
        rdfs:label          "conforms to"@en ;
        rdfs:domain         vf:EconomicResource ;
        rdfs:range          vf:ResourceSpecification ;
        owl:maxCardinality  1 ;
        vs:term_status      "stable" ;
        rdfs:comment        "The primary resource specification or definition of an economic resource."@en ;
        .

vf:containedIn a            owl:ObjectProperty ;
        rdfs:label          "contained in"@en ;
        rdfs:domain         vf:EconomicResource ;
        rdfs:range          vf:EconomicResource ;
        vs:term_status      "unstable" ;
        rdfs:comment        "Used when an economic resource contains units also defined as separate economic resources, for example a tool kit or a package of resources for shipping."@en ;
        .

vf:contains a               owl:ObjectProperty ;
        owl:inverseOf       vf:containedIn ;
        rdfs:label          "contains"@en ;
        rdfs:domain         vf:EconomicResource ;
        rdfs:range          vf:EconomicResource ;
        vs:term_status      "unstable" ;
        rdfs:comment        "An economic resource contains at least one other economic resource, for example a tool kit or package of resources for shipping."@en ;
        .

vf:corrects  a              owl:ObjectProperty ;
        rdfs:label          "corrects"@en ;
        rdfs:domain         vf:EconomicEvent ;
        rdfs:range          vf:EconomicEvent ;
        owl:maxCardinality  1 ;
        vs:term_status      "unstable" ;
        rdfs:comment        "Used when an event was entered incorrectly and needs to be backed out or corrected. (The initial event cannot be changed.)"@en ;
        .

vf:created a                owl:DatatypeProperty ;
        rdfs:seeAlso        dcterms:created ;
        rdfs:label          "created"@en ;
        rdfs:domain         [ owl:unionOf (
                                vf:Agreement
                                vf:Claim
                                vf:Commitment
                                vf:Plan
                                vf:Proposal
                                vf:EconomicEvent ) ] ;
        rdfs:range          xsd:dateTimeStamp ;
        owl:maxCardinality  1 ;
        vs:term_status      "testing" ;
        rdfs:comment        "The date, and time if desired, the information was agreed to or recorded."@en ;
        .

vf:currentCurrencyLocation
        a                   owl:DatatypeProperty ;
        rdfs:label          "current currency location"@en ;
        rdfs:domain         vf:EconomicResource ;
        rdfs:range          xsd:string ;
        owl:maxCardinality  1 ;
        vs:term_status      "unstable" ;
        rdfs:comment        "The current virtual place a currency economic resource is located, for example the address for a bank account, crypto wallet, etc., in a domain standard format."@en ;
        .

vf:currentLocation a        owl:ObjectProperty ;
        rdfs:label          "current location"@en ;
        rdfs:domain         vf:EconomicResource ;
        rdfs:range          vf:SpatialThing ;
        owl:maxCardinality  1 ;
        vs:term_status      "stable" ;
        rdfs:comment        "The current physical location of an economic resource.  Could be at any level of granularity, from a town to an address to a warehouse location.  Usually mappable."@en ;
        .

vf:currentVirtualLocation
        a                   owl:DatatypeProperty ;
        rdfs:label          "current virtual location"@en ;
        rdfs:domain         vf:EconomicResource ;
        rdfs:range          xsd:anyURI ;
        owl:maxCardinality  1 ;
        vs:term_status      "testing" ;
        rdfs:comment        "The current virtual place a digital economic resource is located. Usually used for documents, code, or other electronic resource."@en ;
        .

vf:defaultUnitOfEffort a    owl:ObjectProperty ;
        rdfs:label          "default unit of effort"@en ;
        rdfs:domain         vf:ResourceSpecification ;
        rdfs:range          vf:Unit ;
        owl:maxCardinality  1 ;
        vs:term_status      "testing" ;
        rdfs:comment        "The default unit used for use or work or sometimes cite actions."@en ;
        .

vf:defaultUnitOfResource a  owl:ObjectProperty ;
        rdfs:label          "default unit of resource"@en ;
        rdfs:domain         vf:ResourceSpecification ;
        rdfs:range          vf:Unit ;
        owl:maxCardinality  1 ;
        vs:term_status      "testing" ;
        rdfs:comment        "The default unit used for the resource itself."@en ;
        .

vf:due a                    owl:DatatypeProperty ;
        rdfs:label          "due"@en ;
        rdfs:domain         [ owl:unionOf (
                                vf:Plan
                                vf:Commitment
                                vf:Claim
                                vf:Intent) ] ;
        rdfs:range          xsd:dateTimeStamp ;
        owl:maxCardinality  1 ;
        vs:term_status      "stable" ;
        rdfs:comment        "The date, and time if desired, something is expected to be complete."@en ;
        .

vf:effortQuantity a         owl:ObjectProperty ;
        rdfs:label          "effort quantity"@en ;
        rdfs:domain         [ owl:unionOf (vf:EconomicEvent vf:Commitment vf:Intent vf:RecipeFlow vf:Claim) ] ;
        rdfs:range          vf:Measure ;
        owl:maxCardinality  1 ;
        vs:term_status      "stable" ;
        rdfs:comment        "The amount and unit of the work or use or citation effort-based action. This is often expressed with a time unit, but also could be cycle counts or other measures of effort or usefulness."@en ;
        .

vf:eligibleLocation a       owl:ObjectProperty ;
        rdfs:label          "eligible location"@en ;
        rdfs:domain         vf:Proposal ;
        rdfs:range          vf:SpatialThing ;
        owl:maxCardinality  1 ;
        vs:term_status      "unstable" ;
        rdfs:comment        "Location or area where the proposal is valid."@en ;
        .

vf:expirationDate a         owl:DatatypeProperty ;
        rdfs:label          "expiration date"@en ;
        rdfs:domain         vf:BatchLotRecord ;
        rdfs:range          xsd:dateTimeStamp ;
        owl:maxCardinality  1 ;
        vs:term_status      "testing" ;
        rdfs:comment        "The date after which a resource of this batch or lot should no longer be used or consumed."@en ;
        .

vf:finished  a              owl:DatatypeProperty ;
        rdfs:domain         [ owl:unionOf (vf:Commitment vf:Process vf:Intent vf:Claim) ] ;
        rdfs:label          "finished"@en ;
        rdfs:range          xsd:boolean ;
        owl:maxCardinality  1 ;
        vs:term_status      "stable" ;
        rdfs:comment        "The flow or process is complete or not. This is irrespective of if the original goal has been met, and indicates simply that no more will be done. Default false."@en ;
        .

vf:fulfills  a              owl:ObjectProperty ;
        rdfs:label          "fulfills"@en ;
        rdfs:domain         vf:EconomicEvent ;
        rdfs:range          vf:Commitment ;
        vs:term_status      "testing" ;
        rdfs:comment        "The commitment(s) fulfilled completely or partially by an economic event."@en ;
        .

vf:hasBeginning a           owl:DatatypeProperty ;
        rdfs:subPropertyOf  time:hasBeginning ;
        rdfs:label          "has beginning"@en ;
        rdfs:domain         [ owl:unionOf (
                                vf:Commitment
                                vf:EconomicEvent
                                vf:Intent
                                vf:Proposal
                                vf:Process) ] ;
        rdfs:range          xsd:dateTimeStamp ;
        owl:maxCardinality  1 ;
        vs:term_status      "stable" ;
        rdfs:comment        "The planned or actual beginning date, and time if desired, of a flow or process."@en ;
        .

vf:hasDetailedGeometry a    owl:ObjectProperty ;
        rdfs:label          "currency address"@en ;
        rdfs:domain         vf:SpatialThing ;
        rdfs:range          geosparql:Geometry ;
        vs:term_status      "unstable" ;
        rdfs:comment        "A spatial geometry of any complexity and tooling supported by geosparql."@en ;
        .

vf:hasDuration a            owl:ObjectProperty ;
        rdfs:seeAlso        time:hasDuration ;
        rdfs:label          "has duration"@en ;
        rdfs:domain         [ owl:unionOf (
                                vf:RecipeProcess) ] ;
        rdfs:range          vf:Measure ;
        owl:maxCardinality  1 ;
        vs:term_status      "testing" ;
        rdfs:comment        "The temporal extent of the process."@en ;
        .

vf:hasEnd a                 owl:DatatypeProperty ;
        rdfs:subPropertyOf  time:hasEnd ;
        rdfs:label          "has end"@en ;
        rdfs:domain         [ owl:unionOf (
                                vf:Commitment
                                vf:EconomicEvent
                                vf:Intent
                                vf:Proposal
                                vf:Process) ] ;
        rdfs:range          xsd:dateTimeStamp ;
        owl:maxCardinality  1 ;
        vs:term_status      "stable" ;
        rdfs:comment        "The planned or actual ending date, and time if desired, of a flow or process."@en ;
        .

vf:hasIndependentDemand
        a                   owl:ObjectProperty ;
        owl:inverseOf       vf:independentDemandOf ;
        rdfs:label          "has independent demand"@en ;
        rdfs:range          vf:Commitment  ;
        rdfs:domain         vf:Plan ;
        vs:term_status      "testing" ;
        rdfs:comment        "The commitments and/or intents which this plan was created to deliver on."@en ;
        .

vf:hasInput
        a                   owl:ObjectProperty ;
        owl:inverseOf       vf:inputOf ;
        rdfs:label          "has input"@en ;
        rdfs:domain         vf:Process ;
        rdfs:range          [ owl:unionOf (vf:EconomicEvent vf:Commitment vf:Intent) ] ;
        vs:term_status      "testing" ;
        rdfs:comment        "All the input flows of a process."@en ;
        .

vf:hasNumericalValue a      owl:DatatypeProperty ;
        rdfs:subPropertyOf  om:hasNumericalValue ;
        rdfs:label          "has numerical value"@en ;
        rdfs:domain         vf:Measure ;
        rdfs:range          dtype:numericUnion ;
        owl:maxCardinality  1 ;
        vs:term_status      "stable" ;
        rdfs:comment        "A numeric amount."@en ;
        .

vf:hasOutput
        a                   owl:ObjectProperty ;
        owl:inverseOf       vf:outputOf ;
        rdfs:label          "has output"@en ;
        rdfs:domain         vf:Process ;
        rdfs:range          [ owl:unionOf (vf:EconomicEvent vf:Commitment vf:Intent) ] ;
        vs:term_status      "testing" ;
        rdfs:comment        "All the output flows of a process."@en ;
        .

vf:hasPointInTime a         owl:DatatypeProperty ;
        rdfs:subPropertyOf  time:inXSDDateTimeStamp ;
        rdfs:label          "has point in time"@en ;
        rdfs:domain         [ owl:unionOf (
                                vf:Commitment
                                vf:EconomicEvent
                                vf:Intent) ] ;
        rdfs:range          xsd:dateTimeStamp ;
        owl:maxCardinality  1 ;
        vs:term_status      "stable" ;
        rdfs:comment        "The planned or actual date, and time if desired, of a flow; can be used instead of hasBeginning and hasEnd, if so, hasBeginning and hasEnd should be able to return this value."@en ;
        .

vf:hasRecipeInput
        a                   owl:ObjectProperty ;
        owl:inverseOf       vf:recipeInputOf ;
        rdfs:label          "has recipe input"@en ;
        rdfs:domain         vf:RecipeProcess ;
        rdfs:range          vf:RecipeFlow ;
        vs:term_status      "testing" ;
        rdfs:comment        "All the inputs of a recipe process."@en ;
        .

vf:hasRecipeOutput
        a                   owl:ObjectProperty ;
        owl:inverseOf       vf:recipeOutputOf ;
        rdfs:label          "has recipe output"@en ;
        rdfs:domain         vf:RecipeProcess ;
        rdfs:range          vf:RecipeFlow ;
        vs:term_status      "testing" ;
        rdfs:comment        "All the outputs of a recipe process."@en ;
        .

vf:hasUnit a                owl:ObjectProperty ;
        rdfs:subPropertyOf  om:hasUnit ;
        rdfs:label          "has unit"@en ;
        rdfs:domain         vf:Measure ;
        rdfs:range          vf:Unit ;
        owl:maxCardinality  1 ;
        vs:term_status      "stable" ;
        rdfs:comment        "A standard unit of measure."@en ;
        .

vf:image a                  owl:DatatypeProperty ;
        rdfs:label          "image"@en ;
        rdfs:domain         [ owl:unionOf (
                                vf:Agent
                                vf:EconomicEvent
                                vf:EconomicResource
                                vf:Intent
                                vf:ResourceSpecification
                                vf:ProcessSpecification
                                vf:RecipeProcess) ] ;
        rdfs:range          xsd:anyURI ;
        owl:maxCardinality  1 ;
        vs:term_status      "stable" ;
        rdfs:comment        "The uri to an image relevant to the entity, such as a logo, avatar, photo, diagram, etc."@en ;
        .

vf:imageList a              owl:DatatypeProperty ;
        rdfs:label          "image list"@en ;
        rdfs:domain         [ owl:unionOf (
                                vf:EconomicResource
                                vf:Intent
                                vf:ResourceSpecification) ] ;
        rdfs:range          xsd:anyURI ;
        vs:term_status      "stable" ;
        rdfs:comment        "A comma separated list of uri addresses to images relevant to the resource."@en ;
        .

vf:independentDemandOf
        a                   owl:ObjectProperty ;
        rdfs:label          "independent demand of"@en ;
        rdfs:range          vf:Plan ;
        rdfs:domain         vf:Commitment ;
        owl:maxCardinality  1 ;
        vs:term_status      "testing" ;
        rdfs:comment        "This plan is the way this commitment or intent will be realized."@en ;
        .

vf:inputOf
        a                   owl:ObjectProperty ;
        rdfs:label          "input of"@en ;
        rdfs:domain         [ owl:unionOf (vf:EconomicEvent vf:Commitment vf:Intent) ] ;
        rdfs:range          vf:Process ;
        owl:maxCardinality  1 ;
        vs:term_status      "stable" ;
        rdfs:comment        "Relates an input flow to its process."@en ;
        .

vf:inScopeOf  a             owl:ObjectProperty ;
        rdfs:domain         vf:Process ;
        rdfs:label          "in scope of"@en ;
        rdfs:range          vf:Agent ;
        owl:maxCardinality  1 ;
        vs:term_status      "testing" ;
        rdfs:comment        "Scope here means executed in the context of an agent."@en ;
        .

vf:label a                  owl:DatatypeProperty ;
        rdfs:subPropertyOf  rdfs:label ;
        rdfs:label          "label"@en ;
        rdfs:domain         [ owl:unionOf (
                                vf:Unit
                                vf:Action) ] ;
        rdfs:range          xsd:string ;
        owl:cardinality     1 ;
        vs:term_status      "stable" ;
        rdfs:comment        "The label defined for human readable display."@en ;
        .

vf:lat a                    owl:DatatypeProperty ;
        rdfs:subPropertyOf  geo:lat ;
        rdfs:range          dtype:numericUnion ;
        rdfs:domain         vf:SpatialThing ;
        owl:maxCardinality  1 ;
        vs:term_status      "testing" ;
        rdfs:comment        "The WGS84 latitude of a spatial thing (decimal degrees)." ;
        .

vf:listedIn a               owl:ObjectProperty ;
        rdfs:label          "listed in"@en ;
        rdfs:domain         vf:Proposal ;
        rdfs:range          vf:ProposalList ;
        vs:term_status      "testing" ;
        rdfs:comment        "This proposal is part of these lists of proposals."@en ;
        .

vf:lists a                  owl:ObjectProperty ;
        owl:inverseOf       vf:listedIn ;
        rdfs:label          "lists"@en ;
        rdfs:domain         vf:ProposalList ;
        rdfs:range          vf:Proposal ;
        vs:term_status      "testing" ;
        rdfs:comment        "All the proposals included in this proposal list."@en ;
        .

vf:long a                   owl:DatatypeProperty ;
        rdfs:subPropertyOf  geo:long ;
        rdfs:range          dtype:numericUnion ;
        rdfs:domain         vf:SpatialThing ;
        owl:maxCardinality  1 ;
        vs:term_status      "testing" ;
        rdfs:comment        "The WGS84 longitude of a spatial thing (decimal degrees)." ;
        .

vf:mappableAddress a        owl:DatatypeProperty ;
        rdfs:label          "mappable address"@en ;
        rdfs:domain         vf:SpatialThing ;
        rdfs:range          xsd:string ;
        owl:maxCardinality  1 ;
        vs:term_status      "testing" ;
        rdfs:comment        "A textual address that can be mapped using mapping software."@en ;
        .

vf:mediumOfExchange a       owl:DatatypeProperty ;
        rdfs:label          "medium of exchange"@en ;
        rdfs:domain         vf:ResourceSpecification ;
        rdfs:range          xsd:boolean ;
        owl:maxCardinality  1 ;
        vs:term_status      "testing" ;
        rdfs:comment        "True if the resource is a currency, money, token, credit, etc. used as a medium of exchange.  Default false."@en ;
        .

vf:minimumQuantity a        owl:ObjectProperty ;
        rdfs:label          "minimum quantity"@en ;
        rdfs:domain         vf:Intent ;
        rdfs:range          vf:Measure ;
        owl:maxCardinality  1 ;
        vs:term_status      "testing" ;
        rdfs:comment        "The minimum required order amount and unit of the offered resource."@en ;
        .

vf:name a                   owl:DatatypeProperty ;
        rdfs:label          "name"@en ;
        rdfs:range          xsd:string ;
        rdfs:domain         [ owl:unionOf (
                                vf:SpatialThing
                                vf:Agent
                                vf:Agreement
                                vf:EconomicResource
                                vf:Plan
                                vf:Process
                                vf:ProcessSpecification
                                vf:Proposal
                                vf:Recipe
                                vf:RecipeProcess
                                vf:ResourceSpecification) ] ;
        owl:maxCardinality  1 ;
        vs:term_status      "stable" ;
        rdfs:comment        "An informal or formal textual identifier for an object. Does not imply uniqueness."@en ;
        .

vf:note a                   owl:DatatypeProperty ;
        rdfs:subPropertyOf  skos:note ;
        rdfs:label          "note"@en ;
        rdfs:domain         [ owl:unionOf (
                                vf:Agent
                                vf:Agreement
                                vf:Claim
                                vf:Commitment
                                vf:EconomicEvent
                                vf:EconomicResource
                                vf:ExternalLink
                                vf:Intent
                                vf:Plan
                                vf:Process
                                vf:ProcessSpecification
                                vf:Proposal
                                vf:Recipe
                                vf:RecipeFlow
                                vf:RecipeProcess
                                vf:ResourceSpecification
                                vf:SpatialThing) ] ;
        rdfs:range          xsd:string ;
        owl:maxCardinality  1 ;
        vs:term_status      "stable" ;
        rdfs:comment        "Any useful textual information related to the item."@en ;
        .

vf:ofBatchLot a             owl:ObjectProperty ;
        rdfs:label          "of batch or lot"@en ;
        rdfs:domain         vf:EconomicResource ;
        rdfs:range          vf:BatchLotRecord ;
        owl:maxCardinality  1 ;
        vs:term_status      "testing" ;
        rdfs:comment        "The batch lot record of this resource, if it is a batch or lot resource."@en ;
        .

vf:omUnitIdentifier a       owl:DatatypeProperty ;
        rdfs:label          "om unit identifier"@en ;
        rdfs:domain         vf:Unit ;
        rdfs:range          xsd:anyURI ;
        owl:maxCardinality  1 ;
        vs:term_status      "testing" ;
        rdfs:comment        "The unique identifier of the om unit of measure, for standardization across networks."@en ;
        .

vf:onhandQuantity a         owl:ObjectProperty ;
        rdfs:label          "onhand quantity"@en ;
        rdfs:domain         vf:EconomicResource ;
        rdfs:range          vf:Measure ;
        owl:maxCardinality  1 ;
        vs:term_status      "testing" ;
        rdfs:comment        "The current amount and unit of the economic resource which is under direct control of the agent.  It may be more or less than the accounting quantity. This can be either stored or derived from economic events affecting the resource."@en ;
        .

vf:outputOf
        a                   owl:ObjectProperty ;
        rdfs:label          "output of"@en ;
        rdfs:domain         [ owl:unionOf (vf:EconomicEvent vf:Commitment vf:Intent) ] ;
        rdfs:range          vf:Process ;
        owl:maxCardinality  1 ;
        vs:term_status      "stable" ;
        rdfs:comment        "Relates an output flow to its process."@en ;
        .

vf:planIncludes
        a                   owl:ObjectProperty ;
        owl:inverseOf       vf:plannedWithin ;
        rdfs:label          "plan includes"@en ;
        rdfs:domain         vf:Plan ;
        rdfs:range          [ owl:unionOf (vf:Process vf:Commitment vf:Intent) ] ;
        vs:term_status      "testing" ;
        rdfs:comment        "The processes and non-process commitments/intents that constitute the plan."@en ;
        .

vf:plannedWithin
        a                   owl:ObjectProperty ;
        rdfs:label          "planned within"@en ;
        rdfs:domain         [ owl:unionOf (vf:Process vf:Commitment vf:Intent) ] ;
        rdfs:range          vf:Plan ;
        owl:maxCardinality  1 ;
        vs:term_status      "testing" ;
        rdfs:comment        "The process with its inputs and outputs, or the non-process commitment or intent, is part of the plan."@en ;
        .

vf:primaryAccountable a     owl:ObjectProperty ;
        rdfs:label          "primary accountable"@en ;
        rdfs:domain         vf:EconomicResource ;
        rdfs:range          vf:Agent ;
        owl:maxCardinality  1 ;
        vs:term_status      "stable" ;
        rdfs:comment        "The agent currently with primary rights and responsibilites for the economic resource. It is the agent that is associated with the accountingQuantity of the economic resource."@en ;
        .

vf:primaryLocation a        owl:ObjectProperty ;
        rdfs:label          "primary location"@en ;
        rdfs:domain         vf:Agent ;
        rdfs:range          vf:SpatialThing ;
        owl:maxCardinality  1 ;
        vs:term_status      "testing" ;
        rdfs:comment        "The main place an agent is located, often an address where activities occur and mail can be sent. This is usually a mappable geographic location."@en ;
        .

vf:primaryOutput
        a                   owl:ObjectProperty ;
        rdfs:label          "primary output"@en ;
        rdfs:domain         vf:Recipe ;
        rdfs:range          vf:ResourceSpecification ;
        owl:maxCardinality  1 ;
        vs:term_status      "unstable" ;
        rdfs:comment        "The main output the recipe is intended to produce or deliver."@en ;
        .

vf:processClassifiedAs
        a                   owl:ObjectProperty ;
        rdfs:label          "process classified as"@en ;
        rdfs:domain         vf:RecipeProcess ;
        rdfs:range          xsd:string ;
        vs:term_status      "unstable" ;
        rdfs:comment        "References one or more uri's for a concept in a common taxonomy or other classification scheme for purposes of categorization or grouping; or can be one or more string classifications such as tags."@en ;
        .

vf:processConformsTo
        a                   owl:ObjectProperty ;
        rdfs:label          "process conforms to"@en ;
        rdfs:domain         vf:RecipeProcess ;
        rdfs:range          vf:ProcessSpecification ;
        owl:maxCardinality  1 ;
        vs:term_status      "stable" ;
        rdfs:comment        "The standard specification or definition of a type of process."@en ;
        .

vf:proposedTo
        a                   owl:ObjectProperty ;
        rdfs:label          "proposed to"@en ;
        rdfs:domain         [ owl:unionOf (vf:Proposal vf:ProposalList) ]  ;
        rdfs:range          vf:Agent ;
        vs:term_status      "unstable" ;
        rdfs:comment        "The agent(s) to which the proposal or proposal list is published."@en ;
        .

vf:provider  a              owl:ObjectProperty ;
        rdfs:domain         [ owl:unionOf (vf:EconomicEvent vf:Commitment vf:Intent vf:Claim) ] ;
        rdfs:label          "provider"@en ;
        rdfs:range          vf:Agent ;
        owl:maxCardinality  1 ;
        vs:term_status      "stable" ;
        rdfs:comment        "The economic agent by whom the intended, committed, or actual economic event is initiated."@en ;
        .

vf:publishes
        a                   owl:ObjectProperty ;
        rdfs:label          "publishes"@en ;
        rdfs:domain         vf:Proposal ;
        rdfs:range          vf:Intent ;
        vs:term_status      "testing" ;
        rdfs:comment        "The primary intent(s) of this published proposal. Would be used in intent matching."@en ;
        .

vf:purpose  a               owl:ObjectProperty ;
        rdfs:label          "purpose"@en ;
        rdfs:domain         vf:Proposal ;
        rdfs:range          vf:ProposalPurpose ;
        owl:maxCardinality  1 ;
        vs:term_status      "testing" ;
        rdfs:comment        "The type of proposal, whether offer or request (others may be added as need arises)."@en ;
        .

vf:realizationOf a          owl:ObjectProperty ;
        rdfs:label          "realization of"@en ;
        rdfs:domain         vf:EconomicEvent ;
        rdfs:range          vf:Agreement ;
        owl:maxCardinality  1 ;
        vs:term_status      "stable" ;
        rdfs:comment        "This non-reciprocal economic event occurs as part of this agreement."@en ;
        .

vf:realizes a               owl:ObjectProperty ;
        owl:inverseOf       vf:realizationOf ;
        rdfs:label          "realizes"@en ;
        rdfs:domain         vf:Agreement ;
        rdfs:range          vf:EconomicEvent ;
        vs:term_status      "testing" ;
        rdfs:comment        "All the non-reciprocal economic events (with or without commitments) that realize the agreement."@en ;
        .

vf:realizesReciprocal a     owl:ObjectProperty ;
        owl:inverseOf       vf:reciprocalRealizationOf ;
        rdfs:label          "realizes reciprocal"@en ;
        rdfs:domain         vf:Agreement ;
        rdfs:range          vf:EconomicEvent ;
        vs:term_status      "testing" ;
        rdfs:comment        "All the reciprocal economic events (with or without commitments) that realize the agreement."@en ;
        .

vf:receiver  a              owl:ObjectProperty ;
        rdfs:domain         [ owl:unionOf (vf:EconomicEvent vf:Commitment vf:Intent vf:Claim) ] ;
        rdfs:label          "receiver"@en ;
        rdfs:range          vf:Agent ;
        owl:maxCardinality  1 ;
        vs:term_status      "stable" ;
        rdfs:comment        "The economic agent whom the intended, committed, or actual economic event is for."@en ;
        .

vf:recipeClauseOf
        a                   owl:ObjectProperty ;
        rdfs:label          "recipe clause of"@en ;
        rdfs:domain         vf:RecipeFlow ;
        rdfs:range          vf:RecipeExchange ;
        owl:maxCardinality  1 ;
        vs:term_status      "stable" ;
        rdfs:comment        "Relates a flow to its exchange agreement in a recipe."@en ;
        .

vf:recipeIncludes
        a                   owl:ObjectProperty ;
        rdfs:label          "recipe includes"@en ;
        rdfs:domain         vf:Recipe ;
        rdfs:range          vf:RecipeProcess ;
        vs:term_status      "unstable" ;
        rdfs:comment        "The collection of processes needed for this recipe."@en ;
        .

vf:recipeInputOf
        a                   owl:ObjectProperty ;
        rdfs:label          "recipe input of"@en ;
        rdfs:domain         vf:RecipeFlow ;
        rdfs:range          vf:RecipeProcess ;
        owl:maxCardinality  1 ;
        vs:term_status      "stable" ;
        rdfs:comment        "Relates an input flow to its process in a recipe."@en ;
        .

vf:recipeOutputOf
        a                   owl:ObjectProperty ;
        rdfs:label          "recipe output of"@en ;
        rdfs:domain         vf:RecipeFlow ;
        rdfs:range          vf:RecipeProcess ;
        owl:maxCardinality  1 ;
        vs:term_status      "stable" ;
        rdfs:comment        "Relates an output flow to its process in a recipe."@en ;
        .

vf:recipeReciprocalClauseOf
        a                   owl:ObjectProperty ;
        rdfs:label          "recipe reciprocal clause of"@en ;
        rdfs:domain         vf:RecipeFlow ;
        rdfs:range          vf:RecipeExchange ;
        owl:maxCardinality  1 ;
        vs:term_status      "stable" ;
        rdfs:comment        "Relates a reciprocal flow to its exchange agreement in a recipe."@en ;
        .

vf:recipeStipulates
        a                   owl:ObjectProperty ;
        owl:inverseOf       vf:recipeClauseOf ;
        rdfs:label          "recipe stipulates"@en ;
        rdfs:domain         vf:RecipeExchange ;
        rdfs:range          vf:RecipeFlow ;
        vs:term_status      "testing" ;
        rdfs:comment        "All the primary clauses of a recipe exchange."@en ;
        .

vf:recipeStipulatesReciprocal
        a                   owl:ObjectProperty ;
        owl:inverseOf       vf:recipeReciprocalClauseOf ;
        rdfs:label          "recipe stipulates reciprocal"@en ;
        rdfs:domain         vf:RecipeExchange ;
        rdfs:range          vf:RecipeFlow ;
        vs:term_status      "testing" ;
        rdfs:comment        "All the reciprocal clauses of a recipe exchange."@en ;
        .

vf:reciprocal
        a                   owl:ObjectProperty ;
        rdfs:label          "reciprocal"@en ;
        rdfs:domain         vf:Proposal ;
        rdfs:range          vf:Intent ;
        vs:term_status      "testing" ;
        rdfs:comment        "The reciprocal intent(s) of this published proposal. Not meant to be used for intent matching."@en ;
        .

vf:reciprocalClauseOf a     owl:ObjectProperty ;
        rdfs:label          "reciprocal clause of"@en ;
        rdfs:domain         vf:Commitment ;
        rdfs:range          vf:Agreement ;
        owl:maxCardinality  1 ;
        vs:term_status      "stable" ;
        rdfs:comment        "This commitment is a reciprocal part of the agreement."@en ;
        .

vf:reciprocalRealizationOf
        a                   owl:ObjectProperty ;
        rdfs:label          "reciprocal realization of"@en ;
        rdfs:domain         vf:EconomicEvent ;
        rdfs:range          vf:Agreement ;
        owl:maxCardinality  1 ;
        vs:term_status      "stable" ;
        rdfs:comment        "This reciprocal economic event occurs as part of this agreement."@en ;
        .

vf:resourceClassifiedAs
        a                   owl:ObjectProperty ;
        rdfs:label          "resource classified as"@en ;
        rdfs:domain         [ owl:unionOf (vf:ResourceSpecification vf:RecipeFlow vf:Intent vf:Commitment vf:EconomicEvent vf:Claim) ] ;
        rdfs:range          xsd:string ;
        vs:term_status      "unstable" ;
        rdfs:comment        "References one or more uri's for a concept in a common taxonomy or other classification scheme for purposes of categorization or grouping; or can be one or more string classifications such as tags."@en ;
        .

vf:resourceConformsTo
        a                   owl:ObjectProperty ;
        rdfs:label          "resource conforms to"@en ;
        rdfs:domain         [ owl:unionOf (vf:Commitment vf:Intent vf:EconomicEvent vf:Claim vf:RecipeFlow) ] ;
        rdfs:range          vf:ResourceSpecification ;
        owl:maxCardinality  1 ;
        vs:term_status      "stable" ;
        rdfs:comment        "The lowest level resource specification or definition of an existing or potential economic resource, whether one will ever be instantiated or not."@en ;
        .

vf:resourceInventoriedAs
        a                   owl:ObjectProperty ;
        rdfs:label          "resource inventoried as"@en ;
        rdfs:domain         [ owl:unionOf (vf:Commitment vf:Intent vf:EconomicEvent) ] ;
        rdfs:range          vf:EconomicResource ;
        owl:maxCardinality  1 ;
        vs:term_status      "stable" ;
        rdfs:comment        "Economic resource involved in the flow."@en ;
        .

vf:resourceQuantity a       owl:ObjectProperty ;
        rdfs:label          "resource quantity"@en ;
        rdfs:domain         [ owl:unionOf (vf:EconomicEvent vf:Commitment vf:Intent vf:RecipeFlow vf:Claim) ] ;
        rdfs:range          vf:Measure ;
        owl:maxCardinality  1 ;
        vs:term_status      "stable" ;
        rdfs:comment        "The amount and unit of the economic resource counted or inventoried."@en ;
        .

vf:satisfies
        a                   owl:ObjectProperty ;
        rdfs:label          "satisfies"@en ;
        rdfs:domain         [ owl:unionOf (vf:Commitment vf:EconomicEvent ) ] ;
        rdfs:range          vf:Intent ;
        vs:term_status      "testing" ;
        rdfs:comment        "The intent(s) satisfied fully or partially by an economic event or commitment."@en ;
        .

vf:settles  a               owl:ObjectProperty ;
        rdfs:label          "settles"@en ;
        rdfs:domain         vf:EconomicEvent ;
        rdfs:range          vf:Claim ;
        vs:term_status      "testing" ;
        rdfs:comment        "The claim(s) settled fully or partially by the economic event."@en ;
        .

vf:stage
        a                   owl:ObjectProperty ;
        rdfs:label          "stage"@en ;
        rdfs:domain         [ owl:unionOf (vf:EconomicResource vf:Commitment vf:Intent vf:RecipeFlow) ] ;
        rdfs:range          vf:ProcessSpecification ;
        owl:maxCardinality  1 ;
        vs:term_status      "stable" ;
        rdfs:comment        "The required stage of the desired input economic resource. References the ProcessSpecification of the last process the economic resource went through."@en ;
        .

vf:state
        a                   owl:ObjectProperty ;
        rdfs:label          "state"@en ;
        rdfs:domain         [ owl:unionOf (vf:EconomicResource vf:EconomicEvent vf:RecipeFlow vf:Commitment vf:Intent) ] ;
        rdfs:range          xsd:string ;
        owl:maxCardinality  1 ;
        vs:term_status      "testing" ;
        rdfs:comment        "The required state of the desired input economic resource, after coming out of a test or review process."@en ;
        .

vf:stipulates a             owl:ObjectProperty ;
        owl:inverseOf       vf:clauseOf ;
        rdfs:label          "stipulates"@en ;
        rdfs:domain         vf:Agreement ;
        rdfs:range          vf:Commitment ;
        vs:term_status      "testing" ;
        rdfs:comment        "All the primary commitments that constitute the agreement."@en ;
        .

vf:stipulatesReciprocal a   owl:ObjectProperty ;
        owl:inverseOf       vf:reciprocalClauseOf ;
        rdfs:label          "stipulates reciprocal"@en ;
        rdfs:domain         vf:Agreement ;
        rdfs:range          vf:Commitment ;
        vs:term_status      "testing" ;
        rdfs:comment        "All the reciprocal commitments that constitute the agreement."@en ;
        .

vf:substitutable a          owl:DatatypeProperty ;
        rdfs:label          "substitutable"@en ;
        rdfs:domain         vf:ResourceSpecification ;
        rdfs:range          xsd:boolean ;
        owl:maxCardinality  1 ;
        vs:term_status      "stable" ;
        rdfs:comment        "Defines if any resource of that type can be freely substituted for any other resource of that type when used, consumed, traded, etc."@en ;
        .

vf:symbol a                 owl:DatatypeProperty ;
        rdfs:subPropertyOf  om:symbol ;
        rdfs:label          "symbol"@en ;
        rdfs:domain         vf:Unit ;
        rdfs:range          xsd:string ;
        owl:maxCardinality  1 ;
        vs:term_status      "testing" ;
        rdfs:comment        "The symbol defined for human readable display."@en ;
        .

vf:toLocation a             owl:ObjectProperty ;
        rdfs:label          "to location"@en ;
        rdfs:domain         vf:EconomicEvent ;
        rdfs:range          vf:SpatialThing ;
        owl:maxCardinality  1 ;
        vs:term_status      "testing" ;
        rdfs:comment        "The new location of the receiver resource."@en ;
        .

vf:toResourceInventoriedAs
        a                   owl:ObjectProperty ;
        rdfs:label          "to resource inventoried as"@en ;
        rdfs:domain         vf:EconomicEvent ;
        rdfs:range          vf:EconomicResource ;
        owl:maxCardinality  1 ;
        vs:term_status      "stable" ;
        rdfs:comment        "Additional economic resource on the economic event when needed by the receiver. Used when a transfer or move, or sometimes other actions, requires explicitly identifying an economic resource by the receiver, which is identified differently by the sender."@en ;
        .

vf:trackingIdentifier a     owl:DatatypeProperty ;
        rdfs:label          "tracking identifier"@en ;
        rdfs:domain         vf:EconomicResource ;
        rdfs:range          xsd:string ;
        owl:maxCardinality  1 ;
        vs:term_status      "stable" ;
        rdfs:comment        "Any identifier used to track a singular resource, such as a serial number or VIN."@en ;
        .

vf:triggeredBy  a           owl:ObjectProperty ;
        rdfs:label          "triggered by"@en ;
        rdfs:domain         vf:Claim ;
        rdfs:range          vf:EconomicEvent ;
        owl:maxCardinality  1 ;
        vs:term_status      "testing" ;
        rdfs:comment        "References an economic event that implied the claim, often based on a prior agreement."@en ;
        .

vf:unitBased  a             owl:DatatypeProperty ;
        rdfs:label          "unit based"@en ;
        rdfs:domain         vf:Proposal ;
        rdfs:range          xsd:boolean ;
        owl:maxCardinality  1 ;
        vs:term_status      "testing" ;
        rdfs:comment        "This group of intents contains unit based quantities, which can be multipied to create commitments; commonly seen in a price list or e-commerce. Default false."@en ;
        .

vf:unitOfEffort a           owl:ObjectProperty ;
        rdfs:label          "unit of effort"@en ;
        rdfs:domain         vf:EconomicResource ;
        rdfs:range          vf:Unit ;
        owl:maxCardinality  1 ;
        vs:term_status      "stable" ;
        rdfs:comment        "The unit used for use or work or sometimes cite actions."@en ;
        .
